BPF_CALL symbolic execution

lean/test/bpf/examples/common/helpers.h
@@ -1,0 +1,3 @@
+#pragma once
+
+static int (*bpf_get_prandom_u32)(void) = (void *) 7;
