lean/test/bpf/examples/common/ret-random.c
@@ -1,0 +1,6 @@
+#include <helpers.h>
+
+int main(void) {
+    int x = bpf_get_prandom_u32();
+    return x;
+}
